hybrid_mem/DetMem.v
@@ -16,34 +16,34 @@ Module DetMem. Section DetMem.
       if (bool_decide (0 <= (8 * sz) < modulus_64))%Z
       then (
             let mem0 : Mem.t := mem in
-            let (blk, mem1) := Mem.alloc mem0 sz in
+            let (loc, mem1) := Mem.alloc mem0 sz in
             trigger (SPut v_mem mem1↑);;;
-            Ret (Vptr (blk, 0%Z)))
+            Ret (Vint loc))
       else triggerUB
 . 
 
   Definition free : list val → itree crisE val :=
     λ arg,
-      bofs <- (pargs [Tptr] arg)?;;
+      loc <- (pargs [Tint] arg)?;;
       mem <- trigger (SGet v_mem);; mem <- mem↓?;;
-      mem1 <- (Mem.free mem bofs)?;;
+      mem1 <- (Mem.free mem loc)?;;
       trigger (SPut v_mem mem1↑);;;
       Ret (Vint 0)
   . 
 
   Definition load: list val -> itree crisE val :=
     fun arg =>      
-      bofs <- (pargs [Tptr] arg)?;;        
+      'loc : Z <- (pargs [Tint] arg)?;;
       mem <- trigger (SGet v_mem);; mem <- mem↓?;;
-      v <- (Mem.load mem bofs)?;;
+      v <- (Mem.load mem loc)?;;
       Ret v
   .
 
   Definition store : list val → itree crisE val :=
     fun arg =>
-      '(bofs, v): _ <- (pargs [Tptr; Tuntyped] arg)?;;
+      '(loc, v) : _ <- (pargs [Tint; Tuntyped] arg)?;;
       mem <- trigger (SGet v_mem);; mem <- mem↓?;;
-      mem1 <- (Mem.store mem bofs v)?;;
+      mem1 <- (Mem.store mem loc v)?;;
       trigger (SPut v_mem mem1↑);;;
       Ret (Vint 0)
   .
@@ -58,11 +58,11 @@ Module DetMem. Section DetMem.
 
   Definition cas: list val -> itree crisE val :=
     fun arg =>
-      ' (bofs, (v_old, v_new)): _ <- (pargs [Tptr; Tuntyped; Tuntyped] arg)?;;
-      'v_cur: val <- ccallU MemHdr.load [Vptr bofs];;
+      ' (loc, (v_old, v_new)): _ <- (pargs [Tint; Tuntyped; Tuntyped] arg)?;;
+      'v_cur: val <- ccallU MemHdr.load [Vint loc];;
       'succ: val <- ccallU MemHdr.cmp [v_cur; v_old];;
       (if (bool_decide (succ = (Vint 1)))
-       then ccallU MemHdr.store [Vptr bofs; v_new]
+       then ccallU MemHdr.store [Vint loc; v_new]
        else Ret Vundef);;;
       Ret v_cur
   .
